lang.dfy
@@ -1,12 +1,15 @@
 module lang {
   datatype Term  =
+    | Lit(v : Val)
     | Var(x : string)
     | Add(e : Term, e': Term)
     | Sub(e : Term, e': Term)
     | Or(e : Term, e' : Term)
     | And(e : Term, e' : Term)
+    | Eq(e : Term, e' : Term)
     | Record(em : seq<(string,Term)>)
     | RecordProj(e : Term, f : string)
+    | If(eb : Term, e : Term, e' : Term)
 
   datatype Val = IntVal(v : int) | BoolVal(b : bool) | RecordVal(m : map<string,Val>)
 
