Makefile
@@ -1,0 +1,27 @@
+SOURCES := $(shell find . -name '*.dfy')
+
+clean-test-results:
+	rm -rf TestResults/*.csv TestResults/*.trx
+
+restore-dafny:
+	dotnet tool restore
+
+NUM_ITERATIONS = 100
+
+MEASURE_COMPLEXITY_ARGS = --iterations:$(NUM_ITERATIONS) --log-format csv 
+
+$(SOURCES): restore-dafny clean-test-results
+	-dotnet tool run dafny measure-complexity $(MEASURE_COMPLEXITY_ARGS) $@
+
+stress : $(SOURCES)
+
+clean:
+	rm -rf build
+	rm -rf TestResults/*
+
+
+love:
+	...
+
+war:
+	...
